examples/opaque/client_proofs.v
@@ -18,10 +18,12 @@ Notation iProp := (iProp Σ).
 
 Lemma wp_client_session (uid pw : term) (c : val):
 {{{ cryptis_ctx
-      ∗ hash_pred (opN.@"A_u") (λ _,  True)
+      ∗ hash_pred (opN.@"A_u") A_pred
+      ∗ hash_pred (opN.@"A_s") A_pred
       ∗ hash_pred (opN.@"SK") (λ _,  False)
       ∗ hash_pred (opN.@"K") (λ _,  False)
       ∗ hash_pred (opN.@"α") (λ _,  True)
+      ∗ senc_pred (opN.@"AuthEnc") envelope_pred
       ∗ channel c
       ∗ public uid
       ∗ minted uid
@@ -29,15 +31,13 @@ Lemma wp_client_session (uid pw : term) (c : val):
 Client.session uid c pw
 {{{ x , RET (repr x) ; SK_priv x }}}.
 Proof.
-  iIntros "%ϕ (#Cryptis & #HpredA_u & #HpredSK & #HpredK & #Hpredα & #Hc & #pubuid & #minteduid & #mintedpw) Hhl".
+  iIntros "%ϕ (#Cryptis & #HpredA_u & #HpredA_s & #HpredSK & #HpredK & #Hpredα & #SpredAuth & #Hc & #pubuid & #minteduid & #mintedpw) Hhl".
   wp_lam. wp_pures.
-  wp_apply (wp_mk_nonce (fun _ => False)%I (fun _ => True)%I) => //.
-  iIntros "%x_u %Hnoncex_u #Hmintedx_u #Hprivatex_u #Heqx_u #Hsx_uV #Heqx_uV Htokenx_u".
+  wp_apply (wp_mk_nonce (fun _ => False)%I (fun t => opaque_secret t)%I) => //.
+  iIntros "%x_u %Hnoncex_u #Hmintedx_u #Hprivatex_u #Hexpx_u #? #Hexpx_uV Htokenx_u".
   wp_pures.
   wp_apply (wp_mk_nonce (fun _ => False)%I (fun _ => True)%I) => //.
   iIntros "%r %Hnoncer #Hmintedr #Hprivater #Heqr #HsrV #HeqrV Htokenr".
-  (* iAssert (public (TInv r) ↔ ▷ □ False)%I as "{HsrV} HsrV". *)
-  (* { admit. } *)
   wp_pures.
   wp_apply wp_H'.
   wp_apply wp_texp.
@@ -46,6 +46,7 @@ Proof.
   wp_list.
   wp_term_of_list.
   wp_pures.
+  set m1 := Spec.of_list _.
   wp_apply wp_send => //.
   do !rewrite public_of_list /=.
   do !iSplit => //.
@@ -61,7 +62,7 @@ Proof.
   do !iSplit => //.
   by iApply minted_TInt.
   iApply exp_pred_intro1.
-  by iApply "Heqx_u".
+  by iApply "Hexpx_u"; iPureIntro; rewrite exps_TExpN.
   by rewrite public_TInt; auto.
   wp_pures.
   wp_apply wp_recv => //.
@@ -73,7 +74,7 @@ Proof.
   wp_list_match => [β X_s envelope A_s -> | _].
   1, 2: wp_pures.
   2, 3: by iApply ("Hhl" $! None).
-wp_apply wp_hl_inv_term.
+  wp_apply wp_hl_inv_term.
   wp_apply wp_texp.
   wp_list.
   wp_apply wp_H.
@@ -116,11 +117,16 @@ wp_apply wp_hl_inv_term.
   do !iSplit => //; iApply all_minted_TExp; iSplit => //.
   rewrite minted_THash minted_tag minted_of_list /=.
   do !iSplit => //.
-  rewrite minted_TExp.
+  rewrite [minted (TExp _ r)]minted_TExp.
   iSplit => //.
   by rewrite minted_THash minted_tag.
   by intro contra.
-  2: by wp_pures; iApply ("Hhl" $! None).
+  3: by wp_pures; iApply ("Hhl" $! None).
+  iNext. iModIntro.
+  iExists P_s, p_u, X_s, x_u, (hash_result "ssid'" (Spec.of_list [uid; TExp (hash_result "α" pw) r])).
+  do !iSplit => //.
+  unfold opaque_public_private_pair.
+  admit.
   wp_list.
   wp_pures.
   set SK := hash_result _ _.
@@ -133,13 +139,15 @@ wp_apply wp_hl_inv_term.
   iDestruct "contra" as "[contra _]".
   iDestruct (public_THashE with "HpredK contra") as "[contra | [_ contra]]" => //.
   rewrite public_of_list.
-  iDestruct "contra" as "(_ & contra & _)".
+  iDestruct "contra" as "(contra & _ & _)".
   admit.
   iApply (public_THashIS with "HpredSK") => //.
   rewrite minted_of_list.
   do !iSplit => //; rewrite minted_THash minted_tag minted_of_list; do !iSplit => //.
-  1, 2: rewrite -all_minted_TExp; iSplit => //.
-  rewrite -all_minted_TExp minted_THash minted_tag.
+  1: rewrite -[minted (TExp P_s p_u)]all_minted_TExp.
+  2: rewrite -all_minted_TExp.
+  1, 2: iSplit => //.
+  rewrite -[minted (TExp _ r)] all_minted_TExp minted_THash minted_tag.
   by iSplit => //.
 Admitted.
 
