examples/opaque/server_proofs.v
@@ -25,39 +25,32 @@ Definition opaque_file (file : val) : iProp :=
   ∃ k_s p_s P_s P_u envelope,
     ⌜file = Spec.of_list [k_s; p_s; P_s; P_u; envelope]⌝
     ∗ minted k_s ∗ □(public k_s ↔ ▷ □ False) ∗
-    □(∀ t' : term, exp_pred_base k_s t' ↔ ▷ □ True) ∗
     □(public (TInv k_s) ↔ ▷ False) ∗
+    □(∀ t' : term, exp_pred_base k_s t' ↔ ▷ □ True) ∗
     □(∀ t' : term, exp_pred_base (TInv k_s) t' ↔ ▷ False) ∗
-    minted p_s ∗ □(public p_s ↔ ▷ □ False) ∗
-    □(∀ t' : term, exp_pred_base p_s t' ↔ ▷ □
-                                 ∃ (b: term) e,
-                                   ⌜TExp b e = t'⌝
-                                   ∗ match b with
-                                   | TInt _ => True
-                                   | _ => False
-                                   end) ∗
-    public P_s ∗ public P_u ∗ public envelope.
+    public P_s ∗ public envelope ∗
+    opaque_public_private_pair p_s P_u.
 
 Definition opaque_db (db : gmap term val) : iProp :=
 [∗ map] (k : term) ↦ (file : val) ∈ db,
 public k ∗ opaque_file file.
 
-Lemma wp_make_file (pw : term) (Φ : senc_key → term → iProp) :
+Lemma wp_make_file (pw : term) :
 {{{ cryptis_ctx
     ∗ minted pw
     ∗ □ (public pw ↔ ▷ □ False)
     ∗ hash_pred (opN.@"rw") (λ _,  False)
-    ∗ senc_pred (opN.@"AuthEnc") Φ
-    ∗ □ ∀ s t, Φ s t }}}
+    ∗ senc_pred (opN.@"AuthEnc") envelope_pred
+    }}}
 Server.make_file pw
 {{{ file , RET (repr file) ; opaque_file file }}}.
 Proof.
-  iIntros "%ϕ [#cryptis [#Hmintedpw [#Hprivpw [#Hhashpred [#Hsencpred #Henc]]]]] post".
+  iIntros "%ϕ (#cryptis & #Hmintedpw & #Hprivpw & #Hhashpred & #Hsencpred) post".
   wp_lam.
   wp_apply (wp_mk_nonce (fun _ => False)%I (fun _ => True)%I) => //.
-  iIntros "%k_s %Hnoncek_s #Hmintedk_s #Hprivatek_s #Heqk_s #Hsk_sV #Heqk_sV Htokenk_s".
-  (* iAssert (public (TInv k_s) ↔ ▷ False)%I as "{Hsk_sV} Hsk_sV". *)
-  (* { admit. } *)
+  iIntros "%k_s %Hnoncek_s #Hmintedk_s #Hprivatek_s #Hexpk_s #? #Hexpk_sV Htokenk_s".
+  iAssert (public (TInv k_s) ↔ ▷ False)%I as "Hprivk_sV".
+  admit.
   wp_pures.
   wp_lam.
   wp_pures.
@@ -67,18 +60,33 @@ Proof.
   wp_apply wp_H.
   wp_apply wp_derive_senc_key.
   wp_pures.
-  wp_apply (wp_mk_nonce (fun _ => False)%I
-                      (fun t => ∃ (b: term) e,
-                           ⌜TExp b e = t⌝
-                                         ∗ match b with
-                                           | TInt _ => True
-                                           | _ => False
-                                           end
-                      )%I) => //.
-  iIntros "%p_s %Hnoncep_s #Hmintedp_s #Hprivatep_s #Hexppredp_s #? #Hexppredp_sV Htokenp_s".
+  wp_apply (wp_mk_nonce (fun _ => False)%I opaque_secret) => //.
+  iIntros "%p_s %Hnoncep_s #Hmintedp_s #Hprivatep_s #Hexpp_s #? #Hexpp_sV Htokenp_s".
+  iAssert (public (TInv p_s) ↔ ▷ False)%I as "Hprivp_sV".
+  admit.
   wp_pures.
-  wp_apply (wp_mk_nonce (fun _ => False)%I (fun _ => True)%I) => //.
-  iIntros "%p_u %Hnoncep_u #Hmintedp_u #Hprivatep_u #Heqp_u #? #Heqp_uV Htokenp_u".
+  wp_apply (wp_mk_nonce_fresh {[(TExp g p_s)]} (fun _ => False)%I opaque_secret) => //.
+  - iIntros "%". rewrite elem_of_singleton. iIntros "->".
+    iApply minted_TExp.
+    by intro contra.
+    iSplit => //.
+    by iApply minted_TInt.
+  iIntros "%p_u %Hfreshp_u %Hnoncep_u #Hmintedp_u #Hprivatep_u #Hexpp_u #Hsrp_uV #Hexpp_uV Htokenp_u".
+  iAssert (public (TInv p_u) ↔ ▷ False)%I as "Hprivp_uV".
+  admit.
+  assert (p_u ≠ p_s) as Hneq.
+  intro contra.
+  apply (Hfreshp_u (TExp g p_s)).
+  by rewrite elem_of_singleton.
+  rewrite contra.
+  assert (negb (is_exp g)) as H0.
+  done.
+  assert (invs_canceled [p_s]) as H1.
+  by apply invs_canceled1.
+  assert (subterm p_s p_s) as H2.
+  by apply STRefl.
+  apply (STExp2 H0 H1 H2).
+  by rewrite elem_of_list_singleton.
   wp_pures.
   wp_apply wp_texp. wp_pures.
   wp_apply wp_texp.
@@ -90,25 +98,34 @@ Proof.
   wp_term_of_list.
   iApply "post".
   iExists k_s, p_s, (TExp g p_s), (TExp g p_u), _.
-  do !iSplit => //.     
-  1, 2: iApply public_TExp_iff; auto.
-  1, 2: do !iSplit => //.
-  1, 4: by iApply minted_TInt.
+  do !iSplit => //.
+  iApply public_TExp_iff; auto.
+  do !iSplit => //.
+  by iApply minted_TInt.
   iApply exp_pred_intro1.
-  iApply "Hexppredp_s".
-  iNext. iModIntro.
-  iExists g, p_s.
-  by iSplit => //.
-  1, 3: by rewrite public_TInt; auto.
-  iApply exp_pred_intro1.
-  by iApply "Heqp_u"; auto.
-  iApply (public_sencIS _ (opN.@"AuthEnc") Φ _) => //.
+  iApply "Hexpp_s".
+  by iNext; iModIntro; iPureIntro; rewrite exps_TExpN.
+  by iModIntro; iIntros "?"; iApply public_TInt.
+  iApply (public_sencIS _ (opN.@"AuthEnc") envelope_pred _) => //.
   rewrite minted_senc minted_THash minted_tag.
   1, 2: iApply minted_of_list; do !iSplit => //; iApply minted_TExp.
   1, 3, 5: by intro contra.
   1- 3: iSplit => //.
   by rewrite minted_THash minted_tag.
   1, 2: by iApply minted_TInt.
+  iModIntro.
+  iExists p_u, (TExp g p_u), (TExp g p_s).
+  iSplit => //.
+  iExists p_s.
+  do !iSplit => //.
+  iPureIntro.
+  apply Hfreshp_u.
+  by rewrite elem_of_singleton.
+  iApply public_TExp_exp_pred => //.
+  by iApply public_TInt.
+  iApply exp_pred_intro1.
+  iApply "Hexpp_s".
+  by iNext; iModIntro; iPureIntro; rewrite exps_TExpN.
   iModIntro.
   rewrite public_senc_key.
   iIntros "#Hcompromise".
@@ -117,16 +134,27 @@ Proof.
   iDestruct "Hprivpw" as "[Hprivpw _]".
   iDestruct "Hpub" as "[Hpubpw _]".
   iDestruct ("Hprivpw" with "Hpubpw") as "contra".
-  all: by iDestruct "Hprivatep_u" as "[_ Hprivatep_u]";
-    iDestruct ("Hprivatep_u" with "contra") as "Hpubp_u";
-    iDestruct "Hprivatep_s" as "[_ Hprivatep_s]";
-    iDestruct ("Hprivatep_s" with "contra") as "Hpubp_s";
-    do !iSplit => //; do ?iApply public_TExp => //; rewrite public_TInt.
-Qed.
+  1, 2: by iDestruct "Hprivatep_u" as "[_ Hprivatep_u]";
+  iDestruct ("Hprivatep_u" with "contra") as "Hpubp_u";
+  iDestruct "Hprivatep_s" as "[_ Hprivatep_s]";
+  iDestruct ("Hprivatep_s" with "contra") as "Hpubp_s";
+  do !iSplit => //; do ?iApply public_TExp => //; rewrite public_TInt.
+  iExists p_u.
+  do !iSplit => //.
+  iPureIntro.
+  apply /subtermsP. rewrite subtermsE // cancel_exps1 /g subtermsE /= !right_id_L.
+  rewrite [subterms p_u]subterms_nonce //.
+  admit.
+  iApply public_TExp_exp_pred => //.
+  by iApply public_TInt.
+  iApply exp_pred_intro1.
+  iApply "Hexpp_u".
+  by iNext; iModIntro; iPureIntro; rewrite exps_TExpN.
+Admitted.
 
 Lemma wp_server_session (db c : val) (alist : gmap term val) :
 {{{ cryptis_ctx
-    ∗ hash_pred (opN.@"A_s") (λ _,  True)
+    ∗ hash_pred (opN.@"A_s") A_pred
     ∗ hash_pred (opN.@"SK") (λ _,  False)
     ∗ hash_pred (opN.@"K") (λ _,  False)
     ∗ channel c
@@ -143,7 +171,7 @@ Proof.
   iIntros "%m1 #Hpubm1".
   wp_list_of_term m1; wp_pures.
   2: by iApply ("Hhl" $! None).
-  do !rewrite subst_list_match /=.
+  rewrite !subst_list_match /=.
   wp_list_match => [uid α X_u -> | _].
   2: by wp_pures; iApply ("Hhl" $! None).
   wp_bind (AList.find _ _).
@@ -152,19 +180,25 @@ Proof.
   case db_uid: (alist !! uid) => [file|]; wp_pures.
   2: by iApply ("Hhl" $! None).
   iDestruct ("Hmapcontents" $! uid file with "[//]") as
-  "[_ (%k_s & %p_s & %P_s & %P_u & %envelope &
-        %e & Hmk_s & Hprivk_s & Hexppredk_s & Hexppredk_sV &
-        Hmp_s & Hprivp_s & Hexpp_s & HpP_s & HpP_u & Hpenvelope)]".
+    "[_ (%k_s & %p_s & %P_s & %P_u & %envelope &
+        %e & Hmk_s & Hprivk_s & Hprivk_sV & Hexpk_s & Hexpk_sV &
+        HpubP_s & Hpenvelope & %p_u & %HP_u & %Hfreshp_u &
+        %Hnoncep_s & %Hnoncep_u & HpubP_u & Hminp_s & ? & Hexpp_s & ? & Hprivp_s & ?)]".
   rewrite !subst_list_match /= e.
   wp_apply wp_list_of_term.
   rewrite Spec.of_listK.
   wp_pures.
   rewrite subst_list_match /=.
   wp_list_match => [k_s' p_s' P_s' P_u' envelope' e' | ].
+  symmetry in e'.
   inversion e'. subst. clear e'.
   2: by intro contra.
-  wp_apply (wp_mk_nonce (fun _ => False)%I (fun _ => True)%I) => //.
-  iIntros "%x_s %Hnoncex_s #Hmintedx_s #Hprivatex_s #Hexpx_s #? #Hexpx_sV Htokenx_s".
+  rewrite public_of_list /=.
+  iDestruct "Hpubm1" as "(? & ? & ? & _)".
+  wp_apply (wp_mk_nonce_fresh {[X_u]} (fun _ => False)%I (fun t => opaque_secret t)%I) => //.
+  - iIntros "%". rewrite elem_of_singleton public_minted. iIntros "->".
+    by iApply public_minted.
+  iIntros "%x_s %Hfreshx_s %Hnoncex_s #Hmintedx_s #Hprivatex_s #Hexpx_s #? #Hexpx_sV Htokenx_s".
   wp_pures.
   wp_apply wp_texp. wp_pures.
   wp_apply wp_texp. wp_pures.
@@ -177,26 +211,30 @@ Proof.
   wp_apply wp_prf.
   wp_list.
   wp_term_of_list.
-  rewrite public_of_list => /=.
-  iDestruct "Hpubm1" as "[Hpubuid [Hpubα [HpubX_u _]]]".
   wp_pures.
+  set m2 := (Spec.of_list [_; _; _; _]).
   wp_apply wp_send => //.
   rewrite public_of_list => //.
   do !iSplit => //.
   iApply public_TExp_exp_pred => //.
-  iApply exp_pred_intro1.
-  by iApply "Hexppredk_s".
+  iApply exp_pred_intro1 => //.
+  by iApply "Hexpk_s".
   iApply public_TExp_iff; auto.
   do !iSplit => //.
   by iApply minted_TInt.
   iApply exp_pred_intro1.
-  by iApply "Hexpx_s"; auto.
+  by iApply "Hexpx_s"; iPureIntro; rewrite exps_TExpN.
   by rewrite public_TInt; auto.
   iApply public_THashIS => //.
   rewrite minted_of_list /= !minted_THash !minted_tag !minted_of_list /=.
   do !iSplit => //.
   1, 2: iApply all_minted_TExp; iSplit => //.
   1- 4: by iApply public_minted.
+  iNext. iModIntro.
+  iExists (TExp g p_u), p_s, X_u, x_s, (hash_result "ssid'" (Spec.of_list [uid; α])).
+  do !iSplit => //.  
+  iExists p_u.
+  do !iSplit => //.
   wp_pures.
   wp_apply (wp_recv with "Hc").
   iIntros "%m3 #Hm3pub".
@@ -208,22 +246,28 @@ Proof.
   set SK := hash_result _ _.
   iApply ("Hhl" $! (Some SK)).
   rewrite /SK_priv /SK.
-  iSplit => //.
-  iIntros "Hcontra".
-  iDestruct (public_THashE with "HpredSK Hcontra") as "[Hpub | [_ contra]]" => //.
-  rewrite public_of_list.
+  iSplit; iIntros "contra".
+  iDestruct (public_THashE with "HpredSK contra") as "[Hpub | [_ contra]]" => //.
+  rewrite public_of_list /=.
   iDestruct "Hpub" as "[Hpub _]".
-  iDestruct (public_THashE with "HpredK Hpub") as "[Hpub | [_ contra]]" => //.
-  rewrite public_of_list.
-  iDestruct "Hpub" as "(_ & Hcontra & _)".
-  (* g^ab <-> false*)
-  admit.
-  iIntros "#contra".
+  iDestruct (public_THashE with "HpredK Hpub") as "[Hpub' | [_ contra]]" => //.
+  rewrite public_of_list /=.
+  iDestruct "Hpub'" as "(contra & _)".
+  rewrite TExp_TExpN.
+  have p_s_u: p_s ≠ p_u.
+    move=> p_u_s; apply: Hfreshp_u; rewrite -p_u_s.
+    apply/subtermsP; rewrite subtermsE // cancel_exps1 /=.
+    rewrite [subterms p_s]subterms_nonce //; set_solver.
+  have p_s_uV : p_s ≠ TInv p_u.
+    move=> contra; have: is_inv (TInv p_u).
+      by rewrite is_inv_TInv; case: (p_u) => // in Hnoncep_u *.
+    by rewrite -contra; case: (p_s) => // in Hnoncep_s *.
+  by iApply (public_opaque_secret _ p_s_u p_s_uV).
   iApply (public_THashIS with "HpredSK") => //.
   rewrite minted_of_list.
   do !iSplit => //; rewrite minted_THash minted_tag minted_of_list; do !iSplit => //.
   1, 2: rewrite -all_minted_TExp; iSplit => //.
   all: by iApply public_minted.
-Admitted.
+Qed.
 
 End Opaque.
